Representation spec of `rvector`

ulib/LowStar.RVector.fst
@@ -15,6 +15,16 @@ module V = LowStar.Vector
 
 module U32 = FStar.UInt32
 
+/// Utils
+
+val seq_map_g: 
+  #a:Type0 -> #b:Type0 -> f:(a -> GTot b) -> s:S.seq a -> 
+  GTot (bs:S.seq b{S.length bs = S.length s})
+       (decreases (S.length s))
+let rec seq_map_g #a #b f s =
+  if S.length s = 0 then S.empty
+  else S.cons (f (S.head s)) (seq_map_g f (S.tail s))
+
 /// Regionality
 
 type erid = rid:HH.rid{HST.is_eternal_region rid}
@@ -138,7 +148,7 @@ val rv_elems_reg:
 let rv_elems_reg #a #rg h rv =
   elems_reg h rv 0ul (V.size_of rv)
 
-// The invariant of rvector
+/// The invariant of rvector
 
 val rv_itself_inv:
   #a:Type0 -> #rg:regional a ->
@@ -174,6 +184,31 @@ let rec rv_loc_elems #a #rg h rv i j =
   else loc_union (rv_loc_elems h rv i (j - 1))
 		 (rv_loc_elem h rv (j - 1))
 
+/// Representation
+
+val as_seq_sub:
+  #a:Type0 -> #rg:regional a -> 
+  h:HS.mem -> rv:rvector rg ->
+  i:uint32_t -> j:uint32_t{i <= j && j <= V.size_of rv} ->
+  GTot (s:S.seq (Rgl?.repr rg){S.length s = U32.v j - U32.v i})
+let as_seq_sub #a #rg h rv i j =
+  seq_map_g (Rgl?.r_repr rg h) (S.slice (V.as_seq h rv) (U32.v i) (U32.v j))
+
+val as_seq:
+  #a:Type0 -> #rg:regional a -> 
+  h:HS.mem -> rv:rvector rg ->
+  GTot (s:S.seq (Rgl?.repr rg){S.length s = U32.v (V.size_of rv)})
+let rec as_seq #a #rg h rv =
+  seq_map_g (Rgl?.r_repr rg h) (V.as_seq h rv)
+
+val as_seq_sub_as_seq:
+  #a:Type0 -> #rg:regional a -> 
+  h:HS.mem -> rv:rvector rg ->
+  Lemma (S.equal (as_seq_sub h rv 0ul (V.size_of rv))
+		 (as_seq h rv))
+	[SMTPat (as_seq_sub h rv 0ul (V.size_of rv))]
+let as_seq_sub_as_seq #a #rg h rv = ()
+
 /// Construction
 
 val create_empty:
@@ -193,7 +228,9 @@ private val create_:
       modifies (V.loc_vector_within rv 0ul cidx) h0 h1 /\
       rv_itself_inv h1 rv /\
       elems_inv h1 rv 0ul cidx /\
-      elems_reg h1 rv 0ul cidx))
+      elems_reg h1 rv 0ul cidx /\
+      S.equal (as_seq_sub h1 rv 0ul cidx)
+      	      (S.create (U32.v cidx) (Rgl?.r_repr rg h1 (Rgl?.cv rg)))))
     (decreases (U32.v cidx))
 private let rec create_ #a #rg rv cidx =
   admit ();
@@ -214,9 +251,9 @@ val create_rid:
       modifies (V.loc_vector rv) h0 h1 /\
       rv_inv h1 rv /\
       V.frameOf rv = rid /\
-      V.size_of rv = len))
-      // S.equal (as_seq h1 blen bv) 
-      // 	      (S.create (U32.v len) (S.create (U32.v blen) ia))))
+      V.size_of rv = len /\
+      S.equal (as_seq h1 rv)
+      	      (S.create (U32.v len) (Rgl?.r_repr rg h1 (Rgl?.cv rg)))))
 let create_rid #a rg len rid =
   let vec = V.create_rid len (Rgl?.cv rg) rid in
   create_ #a #rg vec len;
@@ -231,8 +268,8 @@ val create_reserve:
       modifies (V.loc_vector rv) h0 h1 /\
       rv_inv h1 rv /\
       V.frameOf rv = rid /\
-      V.size_of rv = 0ul))
-      // S.equal (as_seq h1 blen bv) S.empty))
+      V.size_of rv = 0ul /\
+      S.equal (as_seq h1 rv) S.empty))
 let create_reserve #a rg len rid =
   V.create_reserve len (Rgl?.cv rg) rid
 
@@ -245,9 +282,9 @@ val create:
       modifies (V.loc_vector rv) h0 h1 /\
       rv_inv h1 rv /\
       MHS.fresh_region (V.frameOf rv) h0 h1 /\
-      V.size_of rv = len))
-      // S.equal (as_seq h1 blen bv)
-      // 	      (S.create (U32.v len) (S.create (U32.v blen) ia))))
+      V.size_of rv = len /\
+      S.equal (as_seq h1 rv)
+      	      (S.create (U32.v len) (Rgl?.r_repr rg h1 (Rgl?.cv rg)))))
 let create #a rg len =
   let nrid = new_region_ HH.root in
   create_rid rg len nrid
@@ -264,13 +301,17 @@ val insert:
 			      (Rgl?.region_of rg v))))
     (ensures (fun h0 irv h1 ->
       V.frameOf rv = V.frameOf irv /\
-      modifies (V.loc_vector rv) h0 h1 /\
-      rv_inv h1 irv))
-      // S.equal (as_seq h1 blen ibv)
-      // 	      (S.snoc (as_seq h0 blen bv) (B.as_seq h0 v))))
+      modifies (loc_union (V.loc_addr_of_vector rv)
+			  (V.loc_vector irv)) h0 h1 /\
+      rv_inv h1 irv /\
+      S.equal (as_seq h1 irv)
+      	      (S.snoc (as_seq h0 rv) (Rgl?.r_repr rg h0 v))))
 let insert #a #rg rv v =
   admit ();
-  V.insert rv v
+  let hh0 = HST.get () in
+  let irv = V.insert rv v in
+  let hh1 = HST.get () in
+  irv
 
 val insert_copy:
   #a:Type0 -> #rg:regional a -> cp:copyable a rg ->
@@ -281,9 +322,9 @@ val insert_copy:
     (ensures (fun h0 irv h1 ->
       V.frameOf rv = V.frameOf irv /\
       modifies (loc_all_regions_from false (V.frameOf rv)) h0 h1 /\
-      rv_inv h1 irv))
-      // S.equal (as_seq h1 blen ibv)
-      // 	      (S.snoc (as_seq h0 blen bv) (B.as_seq h0 v))))
+      rv_inv h1 irv /\
+      S.equal (as_seq h1 irv)
+      	      (S.snoc (as_seq h0 rv) (Rgl?.r_repr rg h0 v))))
 let insert_copy #a #rg cp rv v =
   admit ();
   let nrid = new_region_ (V.frameOf rv) in
@@ -305,9 +346,9 @@ val assign:
 			      (Rgl?.region_of rg v))))
     (ensures (fun h0 _ h1 -> 
       modifies (V.loc_vector rv) h0 h1 /\
-      rv_inv h1 rv))
-      // S.equal (as_seq h1 blen bv)
-      // 	      (S.upd (as_seq h0 blen bv) (U32.v i) (B.as_seq h0 v))))
+      rv_inv h1 rv /\
+      S.equal (as_seq h1 rv)
+      	      (S.upd (as_seq h0 rv) (U32.v i) (Rgl?.r_repr rg h0 v))))
 let assign #a #rg rv i v =
   admit ();
   V.assign rv i v
@@ -321,9 +362,9 @@ val assign_copy:
     (ensures (fun h0 _ h1 -> 
       modifies (loc_region_only 
 	         false (Rgl?.region_of rg (V.get h0 rv i))) h0 h1 /\
-      rv_inv h1 rv))
-      // S.equal (as_seq h1 blen bv)
-      // 	      (S.upd (as_seq h0 blen bv) (U32.v i) (B.as_seq h0 v))))
+      rv_inv h1 rv /\
+      S.equal (as_seq h1 rv)
+      	      (S.upd (as_seq h0 rv) (U32.v i) (Rgl?.r_repr rg h0 v))))
 let assign_copy #a #rg cp rv i v =
   admit ();
   let copy = Cpy?.copy cp in
